[minor] Use Z formatting functions.
Seems to go much much faster!

common/printing.v
@@ -29,7 +29,7 @@ Definition ascii_of_Z (z : Z) : Ascii.ascii :=
 
 Open Scope string_scope.
 
-Fixpoint printZ_aux (fuel : nat) (z : Z) (acc : String.string) : String.string :=
+Fixpoint format_Z_aux (fuel : nat) (z : Z) (acc : String.string) : String.string :=
   match fuel with
   | O => acc
   | S fuel' =>
@@ -37,16 +37,16 @@ Fixpoint printZ_aux (fuel : nat) (z : Z) (acc : String.string) : String.string :
     | (q, r) =>
       match q with
       | Z0 => String.String (ascii_of_Z r) acc
-      | _ => printZ_aux fuel' q (String.String (ascii_of_Z r) acc)
+      | _ => format_Z_aux fuel' q (String.String (ascii_of_Z r) acc)
       end
     end
   end.
 
-Definition printZ z :=
+Definition format_Z z rest :=
   match z with
-  | Z0 => "0"
-  | Zpos _ => printZ_aux (S (Z.to_nat (Z.log2 z))) z String.EmptyString
-  | Zneg _ => String.append "-" (printZ_aux (S (Z.to_nat (Z.log2 z))) (Z.abs z) String.EmptyString)
+  | Z0 => String.append "0" rest
+  | Zpos _ => format_Z_aux (S (Z.to_nat (Z.log2 z))) z rest
+  | Zneg _ => String.append "-" (format_Z_aux (S (Z.to_nat (Z.log2 z))) (Z.abs z) rest)
   end.
 
 Set Implicit Arguments.
